src/QueryStructure/Refinements/Bags/ListBags.v
@@ -13,16 +13,11 @@ Definition ListAsBag_binsert
            (item: TItem) :=
   cons item container.
 
-Fixpoint ListAsBag_bcount
-           {TItem: Type}
-           (beq : HasDecidableEquality TItem)
-           (container: list TItem)
-           (item: TItem) :=
-  match container with
-    | nil            => 0 
-    | cons head tail => (if beq item head then 1 else 0) 
-                      + ListAsBag_bcount beq tail item
-  end.
+Definition ListAsBag_bcount
+           {TItem TSearchTerm: Type}
+           (matcher: TSearchTerm -> TItem -> bool) 
+           (container: list TItem) (search_term: TSearchTerm) :=
+  List.fold_left (fun acc x => acc + if (matcher search_term x) then 1 else 0) container 0.
 
 Lemma List_BagInsertEnumerate :
   forall {TItem: Type},
@@ -31,23 +26,9 @@ Proof.
   firstorder.
 Qed.
 
-Lemma List_BagInsertCount :
-  forall {TItem: Type},
-    BagInsertCount (@id (list TItem)) ListAsBag_binsert ListAsBag_bcount.
-Proof.
-  compute; firstorder.
-Qed.
-
 Lemma List_BagEnumerateEmpty :
   forall {TItem: Type},
     BagEnumerateEmpty id (@nil TItem).
-Proof.
-  firstorder.
-Qed.
-
-Lemma List_BagCountEmpty :
-  forall {TItem},
-    BagCountEmpty (@id (list TItem)) nil ListAsBag_bcount.
 Proof.
   firstorder.
 Qed.
@@ -72,6 +53,34 @@ Proof.
   firstorder.
 Qed.
 
+Require Import Omega.
+Lemma List_BagCountCorrect_aux :
+  forall {TItem TSearchTerm: Type}
+         (matcher: TSearchTerm -> TItem -> bool),
+  forall (container: list TItem) (search_term: TSearchTerm) default,
+    length (List.filter (matcher search_term) container) + default =
+    List.fold_left
+      (fun (acc : nat) (x : TItem) =>
+         acc + (if matcher search_term x then 1 else 0)) 
+      container default.
+Proof.
+  induction container; intros.
+
+  + trivial.
+  + simpl; destruct (matcher search_term a);
+    simpl; rewrite <- IHcontainer; omega. 
+Qed.
+
+Lemma List_BagCountCorrect :
+  forall {TItem TSearchTerm: Type}
+         (matcher: TSearchTerm -> TItem -> bool),
+         BagCountCorrect (ListAsBag_bcount matcher) (ListAsBag_bfind matcher).
+Proof.
+  unfold BagCountCorrect, ListAsBag_bcount, ListAsBag_bfind; intros;
+  pose proof (List_BagCountCorrect_aux matcher container search_term 0) as temp;
+  rewrite plus_0_r in temp; simpl in temp; exact temp.
+Qed.
+
 Instance ListAsBag
          {TItem TSearchTerm: Type}
          (star: TSearchTerm)
@@ -85,11 +94,11 @@ Instance ListAsBag
     benumerate := id;
     bfind      := ListAsBag_bfind matcher;
     binsert    := ListAsBag_binsert;
+    bcount     := ListAsBag_bcount matcher;
     
     binsert_enumerate := List_BagInsertEnumerate;
-    binsert_count     := List_BagInsertCount;
     benumerate_empty  := List_BagEnumerateEmpty;
-    bcount_empty      := List_BagCountEmpty;
     bfind_star        := List_BagFindStar star matcher find_star;
-    bfind_correct     := List_BagFindCorrect matcher
+    bfind_correct     := List_BagFindCorrect matcher;
+    bcount_correct    := List_BagCountCorrect matcher
   |}.
